AwsCryptographicMaterialProviders/dafny/AwsCryptographyKeyStore/src/CreateKeys.dfy
@@ -19,11 +19,11 @@ module CreateKeys {
   import Types = AwsCryptographyKeyStoreTypes
   import DDB = ComAmazonawsDynamodbTypes
   import KMS = ComAmazonawsKmsTypes
-  import UUID
-  import Time
 
   method CreateBranchAndBeaconKeys(
-    branchKeyId: string,
+    input: Types.CreateKeyInput,
+    timestamp: string,
+    branchKeyVersion: string,
     ddbTableName: DDB.TableName,
     logicalKeyStoreName: string,
     kmsConfiguration: Types.KMSConfiguration,
@@ -31,26 +31,244 @@ module CreateKeys {
     kmsClient: KMS.IKMSClient,
     ddbClient: DDB.IDynamoDBClient
   )
-    returns (res: Result<Types.CreateKeyOutput, Types.Error>)
-    requires 0 < |branchKeyId|
+    returns (output: Result<Types.CreateKeyOutput, Types.Error>)
+    requires input.branchKeyIdentifier.Some? && 0 < |input.branchKeyIdentifier.value|
+    requires 0 < |branchKeyVersion|
+    requires ddbClient.Modifies !! kmsClient.Modifies
+
     requires kmsClient.ValidState() && ddbClient.ValidState()
     modifies ddbClient.Modifies, kmsClient.Modifies
     ensures ddbClient.ValidState() && kmsClient.ValidState()
-  {
-    //= aws-encryption-sdk-specification/framework/branch-key-store.md#wrapped-branch-key-creation
-    //# - `timestamp`: a timestamp for the current time.
-    //# This timestamp MUST be in ISO8601 format in UTC, to microsecond precision (e.g. “YYYY-MM-DDTHH:mm:ss.ssssssZ“)
-    var timestamp :- Time.GetCurrentTimeStamp()
-    .MapFailure(e => Types.KeyStoreException(message := e));
 
-    var maybeBranchKeyVersion := UUID.GenerateUUID();
-    //= aws-encryption-sdk-specification/framework/branch-key-store.md#wrapped-branch-key-creation
-    //# - `version`: a new guid. This guid MUST be [version 4 UUID](https://www.ietf.org/rfc/rfc4122.txt)
-    var branchKeyVersion :- maybeBranchKeyVersion
-    .MapFailure(e => Types.KeyStoreException(message := e));
+    //= aws-encryption-sdk-specification/framework/branch-key-store.md#createkey
+    //= type=implication
+    //# This operation MUST create a [branch key](#branch-key) and a [beacon key](#beacon-key) according to
+    //# the [Branch Key and Beacon Key Creation](#branch-key-and-beacon-key-creation) section.
+    ensures output.Success?
+            ==>
+
+              //= aws-encryption-sdk-specification/framework/branch-key-store.md#branch-key-and-beacon-key-creation
+              //= type=implication
+              //# The wrapped Branch Keys, DECRYPT_ONLY and ACTIVE, MUST be created according to [Wrapped Branch Key Creation](#wrapped-branch-key-creation).
+
+              //= aws-encryption-sdk-specification/framework/branch-key-store.md#wrapped-branch-key-creation
+              //= type=implication
+              //# The operation MUST call [AWS KMS API GenerateDataKeyWithoutPlaintext](https://docs.aws.amazon.com/kms/latest/APIReference/API_GenerateDataKeyWithoutPlaintext.html).
+
+              //= aws-encryption-sdk-specification/framework/branch-key-store.md#wrapped-branch-key-creation
+              //= type=implication
+              //# The call to AWS KMS GenerateDataKeyWithoutPlaintext MUST use the configured AWS KMS client to make the call.
+
+              //= aws-encryption-sdk-specification/framework/branch-key-store.md#branch-key-and-beacon-key-creation
+              //= type=implication
+              //# The operation MUST call [AWS KMS API GenerateDataKeyWithoutPlaintext](https://docs.aws.amazon.com/kms/latest/APIReference/API_GenerateDataKeyWithoutPlaintext.html).
+
+              //= aws-encryption-sdk-specification/framework/branch-key-store.md#branch-key-and-beacon-key-creation
+              //= type=implication
+              //# The call to AWS KMS GenerateDataKeyWithoutPlaintext MUST use the configured AWS KMS client to make the call.
+              && |kmsClient.History.GenerateDataKeyWithoutPlaintext| == |old(kmsClient.History.GenerateDataKeyWithoutPlaintext)| + 2
+
+              //= aws-encryption-sdk-specification/framework/branch-key-store.md#wrapped-branch-key-creation
+              //= type=implication
+              //# The operation MUST call AWS KMS GenerateDataKeyWithoutPlaintext with a request constructed as follows:
+              && var decryptOnlyKmsInput := Seq.Last(Seq.DropLast(kmsClient.History.GenerateDataKeyWithoutPlaintext)).input;
+
+              //= aws-encryption-sdk-specification/framework/branch-key-store.md#wrapped-branch-key-creation
+              //= type=implication
+              //# - `KeyId` MUST be the configured `AWS KMS Key ARN` in the [AWS KMS Configuration](#aws-kms-configuration) for this keystore
+              && decryptOnlyKmsInput.KeyId == kmsConfiguration.kmsKeyArn
+
+              //= aws-encryption-sdk-specification/framework/branch-key-store.md#wrapped-branch-key-creation
+              //= type=implication
+              //# - `NumberOfBytes` MUST be 32.
+              && decryptOnlyKmsInput.NumberOfBytes == Some(32)
+
+              && var decryptOnlyEncryptionContext := Structure.DecryptOnlyBranchKeyEncryptionContext(
+                                                       input.branchKeyIdentifier.value,
+                                                       branchKeyVersion,
+                                                       timestamp,
+                                                       logicalKeyStoreName,
+                                                       kmsConfiguration.kmsKeyArn
+                                                     );
+
+              //= aws-encryption-sdk-specification/framework/branch-key-store.md#wrapped-branch-key-creation
+              //= type=implication
+              //# - `EncryptionContext` MUST be the [DECRYPT_ONLY encryption context for branch keys](#decrypt_only-encryption-context).
+              && decryptOnlyKmsInput.EncryptionContext == Some(decryptOnlyEncryptionContext)
+
+              //= aws-encryption-sdk-specification/framework/branch-key-store.md#wrapped-branch-key-creation
+              //= type=implication
+              //# - GenerateDataKeyWithoutPlaintext `GrantTokens` MUST be this keystore's [grant tokens](https://docs.aws.amazon.com/kms/latest/developerguide/concepts.html#grant_token).
+              && decryptOnlyKmsInput.GrantTokens == Some(grantTokens)
+
+              && Seq.Last(Seq.DropLast(kmsClient.History.GenerateDataKeyWithoutPlaintext)).output.Success?
+              && var decryptOnlyKmsOutput := Seq.Last(Seq.DropLast(kmsClient.History.GenerateDataKeyWithoutPlaintext)).output.value;
+              && decryptOnlyKmsOutput.CiphertextBlob.Some?
+
+              //= aws-encryption-sdk-specification/framework/branch-key-store.md#wrapped-branch-key-creation
+              //= type=implication
+              //# The operation MUST call [AWS KMS API ReEncrypt](https://docs.aws.amazon.com/kms/latest/APIReference/API_ReEncrypt.html)
+              //# with a request constructed as follows:
+              && |kmsClient.History.ReEncrypt| == |old(kmsClient.History.ReEncrypt)| + 1
+
+              //= aws-encryption-sdk-specification/framework/branch-key-store.md#wrapped-branch-key-creation
+              //= type=implication
+              //# The operation MUST call [AWS KMS API ReEncrypt](https://docs.aws.amazon.com/kms/latest/APIReference/API_ReEncrypt.html)
+              //# with a request constructed as follows:
+              && var activeKmsInput := Seq.Last(kmsClient.History.ReEncrypt).input;
+
+              //= aws-encryption-sdk-specification/framework/branch-key-store.md#wrapped-branch-key-creation
+              //= type=implication
+              //# - `SourceKeyId` MUST be the configured `AWS KMS Key ARN` in the [AWS KMS Configuration](#aws-kms-configuration) for this keystore
+              && activeKmsInput.SourceKeyId == Some(kmsConfiguration.kmsKeyArn)
+
+              //= aws-encryption-sdk-specification/framework/branch-key-store.md#wrapped-branch-key-creation
+              //= type=implication
+              //# - `DestinationKeyId` MUST be the configured `AWS KMS Key ARN` in the [AWS KMS Configuration](#aws-kms-configuration) for this keystore
+              && activeKmsInput.DestinationKeyId == kmsConfiguration.kmsKeyArn
+
+              //= aws-encryption-sdk-specification/framework/branch-key-store.md#wrapped-branch-key-creation
+              //= type=implication
+              //# - ReEncrypt `GrantTokens` MUST be this keystore's [grant tokens](https://docs.aws.amazon.com/kms/latest/developerguide/concepts.html#grant_token).
+              && activeKmsInput.GrantTokens == Some(grantTokens)
+
+              //= aws-encryption-sdk-specification/framework/branch-key-store.md#wrapped-branch-key-creation
+              //= type=implication
+              //# - `CiphertextBlob` MUST be the wrapped DECRYPT_ONLY Branch Key.
+              && activeKmsInput.CiphertextBlob == decryptOnlyKmsOutput.CiphertextBlob.value
+
+              //= aws-encryption-sdk-specification/framework/branch-key-store.md#wrapped-branch-key-creation
+              //= type=implication
+              //# - `SourceEncryptionContext` MUST be the [DECRYPT_ONLY encryption context for branch keys](#decrypt_only-encryption-context).
+              && activeKmsInput.SourceEncryptionContext == Some(decryptOnlyEncryptionContext)
+
+              //= aws-encryption-sdk-specification/framework/branch-key-store.md#wrapped-branch-key-creation
+              //= type=implication
+              //# - `DestinationEncryptionContext` MUST be the [ACTIVE encryption context for branch keys](#active-encryption-context).
+              && activeKmsInput.DestinationEncryptionContext == Some(Structure.ActiveBranchKeyEncryptionContext(decryptOnlyEncryptionContext))
+
+              //= aws-encryption-sdk-specification/framework/branch-key-store.md#branch-key-and-beacon-key-creation
+              //= type=implication
+              //# The operation MUST call AWS KMS GenerateDataKeyWithoutPlaintext with a request constructed as follows:
+              && var beaconKmsInput := Seq.Last(kmsClient.History.GenerateDataKeyWithoutPlaintext).input;
+
+              //= aws-encryption-sdk-specification/framework/branch-key-store.md#branch-key-and-beacon-key-creation
+              //= type=implication
+              //# - `KeyId` MUST be the configured `AWS KMS Key ARN` in the [AWS KMS Configuration](#aws-kms-configuration) for this keystore
+              && beaconKmsInput.KeyId == kmsConfiguration.kmsKeyArn
+
+              //= aws-encryption-sdk-specification/framework/branch-key-store.md#branch-key-and-beacon-key-creation
+              //= type=implication
+              //# - `NumberOfBytes` MUST be 32.
+              && beaconKmsInput.NumberOfBytes == Some(32)
+
+              //= aws-encryption-sdk-specification/framework/branch-key-store.md#branch-key-and-beacon-key-creation
+              //= type=implication
+              //# - `EncryptionContext` MUST be the [encryption context for beacon keys](#beacon-key-encryption-context).
+              && beaconKmsInput.EncryptionContext == Some(Structure.BeaconKeyEncryptionContext(decryptOnlyEncryptionContext))
+
+              //= aws-encryption-sdk-specification/framework/branch-key-store.md#branch-key-and-beacon-key-creation
+              //= type=implication
+              //# - `GrantTokens` MUST be this keystore's [grant tokens](https://docs.aws.amazon.com/kms/latest/developerguide/concepts.html#grant_token).
+              && activeKmsInput.GrantTokens == Some(grantTokens)
+
+              //= aws-encryption-sdk-specification/framework/branch-key-store.md#createkey
+              //= type=implication
+              //# If creation of the keys are successful,
+              //# the operation MUST call Amazon DynamoDB TransactWriteItems according to the [write key material](#writing-branch-key-and-beacon-key-to-key-store) section.
+
+              && Seq.Last(Seq.DropLast(kmsClient.History.GenerateDataKeyWithoutPlaintext)).output.Success?
+
+              && Seq.Last(kmsClient.History.ReEncrypt).output.Success?
+              && var activeKmsOutput := Seq.Last(kmsClient.History.ReEncrypt).output.value;
+              && activeKmsOutput.CiphertextBlob.Some?
+
+              && Seq.Last(kmsClient.History.GenerateDataKeyWithoutPlaintext).output.Success?
+              && var beaconKmsOutput := Seq.Last(kmsClient.History.GenerateDataKeyWithoutPlaintext).output.value;
+              && beaconKmsOutput.CiphertextBlob.Some?
+
+              //= aws-encryption-sdk-specification/framework/branch-key-store.md#writing-branch-key-and-beacon-key-to-keystore
+              //= type=implication
+              //# To add the branch keys and a beacon key to the keystore the
+              //# operation MUST call [Amazon DynamoDB API TransactWriteItems](https://docs.aws.amazon.com/amazondynamodb/latest/APIReference/API_TransactWriteItems.html).
+
+              //= aws-encryption-sdk-specification/framework/branch-key-store.md#writing-branch-key-and-beacon-key-to-keystore
+              //= type=implication
+              //# The call to Amazon DynamoDB TransactWriteItems MUST use the configured Amazon DynamoDB Client to make the call.
+
+              && |ddbClient.History.TransactWriteItems| == |old(ddbClient.History.TransactWriteItems)| + 1
+
+              //= aws-encryption-sdk-specification/framework/branch-key-store.md#writing-branch-key-and-beacon-key-to-keystore
+              //= type=implication
+              //# The operation MUST call Amazon DynamoDB TransactWriteItems with a request constructed as follows:
+              && var writeNewKey := Seq.Last(ddbClient.History.TransactWriteItems).input;
+
+              && 3 == |writeNewKey.TransactItems|
+
+              && writeNewKey.TransactItems[0].Put.Some?
+              && writeNewKey.TransactItems[0].Put.value.Item == Structure.ToAttributeMap(
+                                                                  decryptOnlyEncryptionContext,
+                                                                  //= aws-encryption-sdk-specification/framework/branch-key-store.md#wrapped-branch-key-creation
+                                                                  //= type=implication
+                                                                  //# If the call to AWS KMS GenerateDataKeyWithoutPlaintext succeeds,
+                                                                  //# the operation MUST use the GenerateDataKeyWithoutPlaintext result `CiphertextBlob`
+                                                                  //# as the wrapped DECRYPT_ONLY Branch Key.
+                                                                  decryptOnlyKmsOutput.CiphertextBlob.value)
+
+              && writeNewKey.TransactItems[1].Put.Some?
+              && writeNewKey.TransactItems[1].Put.value.Item == Structure.ToAttributeMap(
+                                                                  Structure.ActiveBranchKeyEncryptionContext(decryptOnlyEncryptionContext),
+                                                                  //= aws-encryption-sdk-specification/framework/branch-key-store.md#wrapped-branch-key-creation
+                                                                  //= type=implication
+                                                                  //# If the call to AWS KMS ReEncrypt succeeds,
+                                                                  //# the operation MUST use the ReEncrypt result `CiphertextBlob`
+                                                                  //# as the wrapped ACTIVE Branch Key.
+                                                                  activeKmsOutput.CiphertextBlob.value)
+
+              && writeNewKey.TransactItems[2].Put.Some?
+              && writeNewKey.TransactItems[2].Put.value.Item == Structure.ToAttributeMap(
+                                                                  Structure.BeaconKeyEncryptionContext(decryptOnlyEncryptionContext),
+                                                                  //= aws-encryption-sdk-specification/framework/branch-key-store.md#branch-key-and-beacon-key-creation
+                                                                  //= type=implication
+                                                                  //# If the call to AWS KMS GenerateDataKeyWithoutPlaintext succeeds,
+                                                                  //# the operation MUST use the `CiphertextBlob` as the wrapped Beacon Key.
+                                                                  beaconKmsOutput.CiphertextBlob.value)
+
+              && Seq.Last(ddbClient.History.TransactWriteItems).output.Success?
+
+              //= aws-encryption-sdk-specification/framework/branch-key-store.md#createkey
+              //= type=implication
+              //# If writing to the keystore succeeds,
+              //# the operation MUST return the branch-key-id that maps to both
+              //# the branch key and the beacon key.
+              && output.value.branchKeyIdentifier == input.branchKeyIdentifier.value
+
+
+    //= aws-encryption-sdk-specification/framework/branch-key-store.md#createkey
+    //= type=implication
+    //# Otherwise, this operation MUST yield an error.
+    ensures
+
+      || (&& |kmsClient.History.GenerateDataKeyWithoutPlaintext| == |old(kmsClient.History.GenerateDataKeyWithoutPlaintext)| + 1
+          && Seq.Last(kmsClient.History.GenerateDataKeyWithoutPlaintext).output.Failure?
+          ==> output.Failure?)
+
+      || (&& |kmsClient.History.ReEncrypt| == |old(kmsClient.History.ReEncrypt)| + 1
+          && Seq.Last(kmsClient.History.ReEncrypt).output.Failure?
+          ==> output.Failure?)
+
+      || (&& |kmsClient.History.GenerateDataKeyWithoutPlaintext| == |old(kmsClient.History.GenerateDataKeyWithoutPlaintext)| + 2
+          && Seq.Last(kmsClient.History.GenerateDataKeyWithoutPlaintext).output.Failure?
+          ==> output.Failure?)
+
+      || (&& |ddbClient.History.TransactWriteItems| == |old(ddbClient.History.TransactWriteItems)| + 1
+          && Seq.Last(ddbClient.History.TransactWriteItems).output.Failure?
+          ==> output.Failure?)
+
+  {
 
     var decryptOnlyEncryptionContext := Structure.DecryptOnlyBranchKeyEncryptionContext(
-      branchKeyId,
+      input.branchKeyIdentifier.value,
       branchKeyVersion,
       timestamp,
       logicalKeyStoreName,
@@ -80,11 +298,12 @@ module CreateKeys {
       kmsClient
     );
 
-    var decryptOnlyBranchKeyItem: Structure.VersionBranchKeyItem := Structure.ToAttributeMap(
+
+    var decryptOnlyBranchKeyItem := Structure.ToAttributeMap(
       decryptOnlyEncryptionContext,
       wrappedDecryptOnlyBranchKey.CiphertextBlob.value
     );
-    var activeBranchKeyItem: Structure.ActiveBranchKeyItem := Structure.ToAttributeMap(
+    var activeBranchKeyItem := Structure.ToAttributeMap(
       activeEncryptionContext,
       wrappedActiveBranchKey.CiphertextBlob.value
     );
@@ -101,13 +320,16 @@ module CreateKeys {
       ddbClient
     );
 
-    res := Success(Types.CreateKeyOutput(
-                     branchKeyIdentifier := branchKeyId
-                   ));
+    output := Success(
+      Types.CreateKeyOutput(
+        branchKeyIdentifier := input.branchKeyIdentifier.value
+      ));
   }
 
   method VersionActiveBranchKey(
     input: Types.VersionKeyInput,
+    timestamp: string,
+    branchKeyVersion: string,
     ddbTableName: DDB.TableName,
     logicalKeyStoreName: string,
     kmsConfiguration: Types.KMSConfiguration,
@@ -115,27 +337,262 @@ module CreateKeys {
     kmsClient: KMS.IKMSClient,
     ddbClient: DDB.IDynamoDBClient
   )
-    returns (res: Result<(), Types.Error>)
-    requires 0 < |input.branchKeyIdentifier|
+    returns (output: Result<Types.VersionKeyOutput, Types.Error>)
+    requires 0 < |input.branchKeyIdentifier| && 0 < |branchKeyVersion|
+    requires ddbClient.Modifies !! kmsClient.Modifies
+
     requires kmsClient.ValidState() && ddbClient.ValidState()
     modifies ddbClient.Modifies, kmsClient.Modifies
     ensures ddbClient.ValidState() && kmsClient.ValidState()
+
+
+    ensures output.Success?
+            ==>
+              //= aws-encryption-sdk-specification/framework/branch-key-store.md#versionkey
+              //= type=implication
+              //# VersionKey MUST first get the active version for the branch key from the keystore
+              //# by calling AWS DDB `GetItem`
+              //# using the `branch-key-id` as the Partition Key and `"branch:ACTIVE"` value as the Sort Key.
+              && |ddbClient.History.GetItem| == |old(ddbClient.History.GetItem)| + 1
+              && Seq.Last(ddbClient.History.GetItem).input.Key
+                 == map[
+                      Structure.BRANCH_KEY_IDENTIFIER_FIELD := DDB.AttributeValue.S(input.branchKeyIdentifier),
+                      Structure.TYPE_FIELD := DDB.AttributeValue.S(Structure.BRANCH_KEY_ACTIVE_TYPE)
+                    ]
+
+              && Seq.Last(ddbClient.History.GetItem).output.Success?
+              && Seq.Last(ddbClient.History.GetItem).output.value.Item.Some?
+              && var oldActiveItem := Seq.Last(ddbClient.History.GetItem).output.value.Item.value;
+              && Structure.BranchKeyItem?(oldActiveItem)
+              && Structure.BRANCH_KEY_ACTIVE_VERSION_FIELD in oldActiveItem
+
+              && KMSKeystoreOperations.AttemptKmsOperation?(kmsConfiguration, Structure.ToBranchKeyContext(oldActiveItem, logicalKeyStoreName))
+
+              //= aws-encryption-sdk-specification/framework/branch-key-store.md#versionkey
+              //= type=implication
+              //# The values on the AWS DDB response item
+              //# MUST be authenticated according to [authenticating a keystore item](#authenticating-a-keystore-item).
+
+              //= aws-encryption-sdk-specification/framework/branch-key-store.md#authenticating-a-keystore-item
+              //= type=implication
+              //# The operation MUST use the configured `KMS SDK Client` to authenticate the value of the keystore item.
+              && |kmsClient.History.ReEncrypt| == |old(kmsClient.History.ReEncrypt)| + 2 // This 2 because we need to wrap the new version
+
+              //= aws-encryption-sdk-specification/framework/branch-key-store.md#authenticating-a-keystore-item
+              //= type=implication
+              //# The operation MUST call [AWS KMS API ReEncrypt](https://docs.aws.amazon.com/kms/latest/APIReference/API_ReEncrypt.html)
+              //# with a request constructed as follows:
+              && var reEncryptInput := Seq.Last(Seq.DropLast(kmsClient.History.ReEncrypt)).input;
+
+              //= aws-encryption-sdk-specification/framework/branch-key-store.md#authenticating-a-keystore-item
+              //= type=implication
+              //# - `SourceEncryptionContext` MUST be the [encryption context](#encryption-context) constructed above
+              && reEncryptInput.SourceEncryptionContext == Some(Structure.ToBranchKeyContext(oldActiveItem, logicalKeyStoreName))
+
+              //= aws-encryption-sdk-specification/framework/branch-key-store.md#authenticating-a-keystore-item
+              //= type=implication
+              //# - `SourceKeyId` MUST be the configured `AWS KMS Key ARN` in the [AWS KMS Configuration](#aws-kms-configuration) for this keystore
+              && reEncryptInput.SourceKeyId == Some(kmsConfiguration.kmsKeyArn)
+
+              //= aws-encryption-sdk-specification/framework/branch-key-store.md#authenticating-a-keystore-item
+              //= type=implication
+              //# - `CiphertextBlob` MUST be the `enc` attribute value on the AWS DDB response item
+              && reEncryptInput.CiphertextBlob == oldActiveItem[Structure.BRANCH_KEY_FIELD].B
+
+              //= aws-encryption-sdk-specification/framework/branch-key-store.md#authenticating-a-keystore-item
+              //= type=implication
+              //# - `GrantTokens` MUST be the configured [grant tokens](https://docs.aws.amazon.com/kms/latest/developerguide/concepts.html#grant_token).
+              && reEncryptInput.GrantTokens == Some(grantTokens)
+
+              //= aws-encryption-sdk-specification/framework/branch-key-store.md#authenticating-a-keystore-item
+              //= type=implication
+              //# - `DestinationKeyId` MUST be the configured `AWS KMS Key ARN` in the [AWS KMS Configuration](#aws-kms-configuration) for this keystore
+              && reEncryptInput.DestinationKeyId == kmsConfiguration.kmsKeyArn
+
+              //= aws-encryption-sdk-specification/framework/branch-key-store.md#authenticating-a-keystore-item
+              //= type=implication
+              //# - `DestinationEncryptionContext` MUST be the [encryption context](#encryption-context) constructed above
+              && reEncryptInput.DestinationEncryptionContext == Some(Structure.ToBranchKeyContext(oldActiveItem, logicalKeyStoreName))
+
+
+
+              //= aws-encryption-sdk-specification/framework/branch-key-store.md#versionkey
+              //= type=implication
+              //# The wrapped Branch Keys, DECRYPT_ONLY and ACTIVE, MUST be created according to [Wrapped Branch Key Creation](#wrapped-branch-key-creation).
+
+              && |kmsClient.History.GenerateDataKeyWithoutPlaintext| == |old(kmsClient.History.GenerateDataKeyWithoutPlaintext)| + 1
+
+              //= aws-encryption-sdk-specification/framework/branch-key-store.md#wrapped-branch-key-creation
+              //= type=implication
+              //# The operation MUST call AWS KMS GenerateDataKeyWithoutPlaintext with a request constructed as follows:
+              && var decryptOnlyKmsInput := Seq.Last(kmsClient.History.GenerateDataKeyWithoutPlaintext).input;
+
+              //= aws-encryption-sdk-specification/framework/branch-key-store.md#wrapped-branch-key-creation
+              //= type=implication
+              //# - `KeyId` MUST be the configured `AWS KMS Key ARN` in the [AWS KMS Configuration](#aws-kms-configuration) for this keystore
+              && decryptOnlyKmsInput.KeyId == kmsConfiguration.kmsKeyArn
+
+              //= aws-encryption-sdk-specification/framework/branch-key-store.md#wrapped-branch-key-creation
+              //= type=implication
+              //# - `NumberOfBytes` MUST be 32.
+              && decryptOnlyKmsInput.NumberOfBytes == Some(32)
+
+              && var decryptOnlyEncryptionContext := Structure.NewVersionFromActiveBranchKeyEncryptionContext(
+                                                       Structure.ToBranchKeyContext(oldActiveItem, logicalKeyStoreName),
+                                                       branchKeyVersion,
+                                                       timestamp
+                                                     );
+
+              //= aws-encryption-sdk-specification/framework/branch-key-store.md#wrapped-branch-key-creation
+              //= type=implication
+              //# - `EncryptionContext` MUST be the [DECRYPT_ONLY encryption context for branch keys](#decrypt_only-encryption-context).
+              && decryptOnlyKmsInput.EncryptionContext == Some(decryptOnlyEncryptionContext)
+
+              //= aws-encryption-sdk-specification/framework/branch-key-store.md#wrapped-branch-key-creation
+              //= type=implication
+              //# - GenerateDataKeyWithoutPlaintext `GrantTokens` MUST be this keystore's [grant tokens](https://docs.aws.amazon.com/kms/latest/developerguide/concepts.html#grant_token).
+              && decryptOnlyKmsInput.GrantTokens == Some(grantTokens)
+
+              && Seq.Last(kmsClient.History.GenerateDataKeyWithoutPlaintext).output.Success?
+              && var decryptOnlyKmsOutput := Seq.Last(kmsClient.History.GenerateDataKeyWithoutPlaintext).output.value;
+              && decryptOnlyKmsOutput.CiphertextBlob.Some?
+
+              //= aws-encryption-sdk-specification/framework/branch-key-store.md#wrapped-branch-key-creation
+              //= type=implication
+              //# The operation MUST call [AWS KMS API ReEncrypt](https://docs.aws.amazon.com/kms/latest/APIReference/API_ReEncrypt.html)
+              //# with a request constructed as follows:
+              && |kmsClient.History.ReEncrypt| == |old(kmsClient.History.ReEncrypt)| + 2 // This 2 because we need to wrap the new version
+
+              //= aws-encryption-sdk-specification/framework/branch-key-store.md#wrapped-branch-key-creation
+              //= type=implication
+              //# The operation MUST call [AWS KMS API ReEncrypt](https://docs.aws.amazon.com/kms/latest/APIReference/API_ReEncrypt.html)
+              //# with a request constructed as follows:
+              && var activeKmsInput := Seq.Last(kmsClient.History.ReEncrypt).input;
+
+              //= aws-encryption-sdk-specification/framework/branch-key-store.md#wrapped-branch-key-creation
+              //= type=implication
+              //# - `SourceKeyId` MUST be the configured `AWS KMS Key ARN` in the [AWS KMS Configuration](#aws-kms-configuration) for this keystore
+              && activeKmsInput.SourceKeyId == Some(kmsConfiguration.kmsKeyArn)
+
+              //= aws-encryption-sdk-specification/framework/branch-key-store.md#wrapped-branch-key-creation
+              //= type=implication
+              //# - `DestinationKeyId` MUST be the configured `AWS KMS Key ARN` in the [AWS KMS Configuration](#aws-kms-configuration) for this keystore
+              && activeKmsInput.DestinationKeyId == kmsConfiguration.kmsKeyArn
+
+              //= aws-encryption-sdk-specification/framework/branch-key-store.md#wrapped-branch-key-creation
+              //= type=implication
+              //# - ReEncrypt `GrantTokens` MUST be this keystore's [grant tokens](https://docs.aws.amazon.com/kms/latest/developerguide/concepts.html#grant_token).
+              && activeKmsInput.GrantTokens == Some(grantTokens)
+
+              //= aws-encryption-sdk-specification/framework/branch-key-store.md#wrapped-branch-key-creation
+              //= type=implication
+              //# - `CiphertextBlob` MUST be the wrapped DECRYPT_ONLY Branch Key.
+              && activeKmsInput.CiphertextBlob == decryptOnlyKmsOutput.CiphertextBlob.value
+
+              //= aws-encryption-sdk-specification/framework/branch-key-store.md#wrapped-branch-key-creation
+              //= type=implication
+              //# - `SourceEncryptionContext` MUST be the [DECRYPT_ONLY encryption context for branch keys](#decrypt_only-encryption-context).
+              && activeKmsInput.SourceEncryptionContext == Some(decryptOnlyEncryptionContext)
+
+              //= aws-encryption-sdk-specification/framework/branch-key-store.md#wrapped-branch-key-creation
+              //= type=implication
+              //# - `DestinationEncryptionContext` MUST be the [ACTIVE encryption context for branch keys](#active-encryption-context).
+              && activeKmsInput.DestinationEncryptionContext == Some(Structure.ActiveBranchKeyEncryptionContext(decryptOnlyEncryptionContext))
+
+              && Seq.Last(kmsClient.History.ReEncrypt).output.Success?
+              && var activeKmsOutput := Seq.Last(kmsClient.History.ReEncrypt).output.value;
+              && activeKmsOutput.CiphertextBlob.Some?
+
+              //= aws-encryption-sdk-specification/framework/branch-key-store.md#versionkey
+              //= type=implication
+              //# The call to Amazon DynamoDB TransactWriteItems MUST use the configured Amazon DynamoDB Client to make the call.
+
+              //= aws-encryption-sdk-specification/framework/branch-key-store.md#versionkey
+              //= type=implication
+              //# To add the new branch key to the keystore,
+              //# the operation MUST call [Amazon DynamoDB API TransactWriteItems](https://docs.aws.amazon.com/amazondynamodb/latest/APIReference/API_TransactWriteItems.html).
+              && |ddbClient.History.TransactWriteItems| == |old(ddbClient.History.TransactWriteItems)| + 1
+
+              //= aws-encryption-sdk-specification/framework/branch-key-store.md#versionkey
+              //= type=implication
+              //# The operation MUST call Amazon DynamoDB TransactWriteItems with a request constructed as follows:
+              && var writeNewKey := Seq.Last(ddbClient.History.TransactWriteItems).input;
+
+              && 2 == |writeNewKey.TransactItems|
+
+              && writeNewKey.TransactItems[0].Put.Some?
+              && writeNewKey.TransactItems[0].Put.value.Item == Structure.ToAttributeMap(
+                                                                  decryptOnlyEncryptionContext,
+
+                                                                  decryptOnlyKmsOutput.CiphertextBlob.value)
+
+              && writeNewKey.TransactItems[1].Put.Some?
+              && writeNewKey.TransactItems[1].Put.value.Item == Structure.ToAttributeMap(
+                                                                  Structure.ActiveBranchKeyEncryptionContext(decryptOnlyEncryptionContext),
+
+                                                                  activeKmsOutput.CiphertextBlob.value)
+
+              && Seq.Last(ddbClient.History.TransactWriteItems).output.Success?
+
+              //= aws-encryption-sdk-specification/framework/branch-key-store.md#versionkey
+              //= type=implication
+              //# If DDB TransactWriteItems is successful, this operation MUST return a successful response containing no additional data.
+              && output == Success(Types.VersionKeyOutput)
+
+    ensures
+      //= aws-encryption-sdk-specification/framework/branch-key-store.md#versionkey
+      //= type=implication
+      //# The the item fails to authenticate this operation MUST fail.
+      || (&& |kmsClient.History.ReEncrypt| == |old(kmsClient.History.ReEncrypt)| + 1
+          && Seq.Last(kmsClient.History.ReEncrypt).output.Failure?
+          ==> output.Failure?)
+
+      //= aws-encryption-sdk-specification/framework/branch-key-store.md#versionkey
+      //= type=implication
+      //# Otherwise, this operation MUST yield an error.
+
+      || (&& |kmsClient.History.GenerateDataKeyWithoutPlaintext| == |old(kmsClient.History.GenerateDataKeyWithoutPlaintext)| + 1
+          && Seq.Last(kmsClient.History.GenerateDataKeyWithoutPlaintext).output.Failure?
+          ==> output.Failure?)
+
+      || (&& |kmsClient.History.ReEncrypt| == |old(kmsClient.History.ReEncrypt)| + 2
+          && Seq.Last(kmsClient.History.ReEncrypt).output.Failure?
+          ==> output.Failure?)
+
+      || (&& |ddbClient.History.TransactWriteItems| == |old(ddbClient.History.TransactWriteItems)| + 1
+          && Seq.Last(ddbClient.History.TransactWriteItems).output.Failure?
+          ==> output.Failure?)
+
   {
 
-    var timestamp :- Time.GetCurrentTimeStamp()
-    .MapFailure(e => Types.KeyStoreException(message := e));
-
-    var maybeBranchKeyVersion := UUID.GenerateUUID();
-    var branchKeyVersion :- maybeBranchKeyVersion
-    .MapFailure(e => Types.KeyStoreException(message := e));
-
-    var decryptOnlyEncryptionContext := Structure.DecryptOnlyBranchKeyEncryptionContext(
+    var oldActiveItem :- DDBKeystoreOperations.GetActiveBranchKeyItem(
       input.branchKeyIdentifier,
-      branchKeyVersion,
-      timestamp,
-      logicalKeyStoreName,
-      kmsConfiguration.kmsKeyArn
+      ddbTableName,
+      ddbClient
     );
+
+    var oldActiveEncryptionContext := Structure.ToBranchKeyContext(oldActiveItem, logicalKeyStoreName);
+
+    :- Need(
+      && KMSKeystoreOperations.AttemptKmsOperation?(kmsConfiguration, oldActiveEncryptionContext),
+      Types.KeyStoreException(
+        message := "Wrapping AWS KMS key in dynamodb does not match configured AWS KMS information."));
+
+    var _ :- KMSKeystoreOperations.ReEncryptKey(
+      oldActiveItem[Structure.BRANCH_KEY_FIELD].B,
+      oldActiveEncryptionContext,
+      oldActiveEncryptionContext,
+      kmsConfiguration,
+      grantTokens,
+      kmsClient
+    );
+
+    var decryptOnlyEncryptionContext := Structure.NewVersionFromActiveBranchKeyEncryptionContext(
+      oldActiveEncryptionContext,
+      branchKeyVersion,
+      timestamp
+    );
+
     var activeEncryptionContext := Structure.ActiveBranchKeyEncryptionContext(decryptOnlyEncryptionContext);
 
     var wrappedDecryptOnlyBranchKey :- KMSKeystoreOperations.GenerateKey(
@@ -169,7 +626,9 @@ module CreateKeys {
       ddbClient
     );
 
-    res := Success(());
+    assert && |ddbClient.History.TransactWriteItems| == |old(ddbClient.History.TransactWriteItems)| + 1;
+
+    output := Success(Types.VersionKeyOutput());
   }
 
 }
